theories/Confluence.v
@@ -1,0 +1,102 @@
+From Coq Require Import Relations.Relation_Definitions.
+From Coq Require Import Relations.Relation_Operators.
+Require Import MyRelations.
+
+From Autosubst Require Import Autosubst.
+
+From Coq Require Import List.
+Import ListNotations.
+
+Require Import LambdaM IsCanonical.
+
+(* Confluence of multistep_H in LambdaM *)
+(* ------------------------------------ *)
+
+Lemma capp_assoc t u l u' l' (it: is_canonical t):
+  capp (capp t u l) u' l' = capp t u (l++u'::l').
+Proof.
+  destruct it ; simpl ; try reflexivity.
+  - now rewrite<- app_assoc.
+  - now rewrite<- app_assoc.
+Qed.
+
+Lemma step_H_collapse :
+  (forall t t', step_H t t' -> h t = h t')
+  /\
+  (forall l l', step_H' l l' -> map h l = map h l').
+Proof.
+  apply mut_comp_ind ; intros ; simpl ; try now f_equal.
+  - inversion b. subst. simpl. rewrite capp_assoc.
+    + now rewrite map_app. 
+    + apply h_is_canonical.
+Qed.
+
+Corollary multistep_H_collapse t t' :
+  multistep_H t t' -> h t = h t'.
+Proof.
+  induction 1 as [u | u u1 u2].
+  - reflexivity.
+  - rewrite<- IHclos_refl_trans_1n. now apply step_H_collapse.
+Qed.
+
+Corollary H_confluence t t1 t2 :
+  multistep_H t t1 -> multistep_H t t2 ->
+  exists t', multistep_H t1 t' /\ multistep_H t2 t'. 
+Proof.
+  intros Ht1 Ht2. exists (h t). split.
+  - apply multistep_H_collapse in Ht1. rewrite Ht1.
+    apply h_is_multistep_H.
+  - apply multistep_H_collapse in Ht2. rewrite Ht2.
+    apply h_is_multistep_H.
+Qed.
+
+(* Given the confluence of the STLC, we may even prove
+ confluence in the canonical subsystem and in LambdaM! *)
+(* --------------------------------------------------- *)
+
+Require Import Lambda LambdaIsomorphism
+  CanonicalIsomorphism Conservativeness.
+
+Section Confluence.
+  Hypothesis Lambda_confluence : forall s s1 s2,
+      Lambda.multistep s s1 -> Lambda.multistep s s2 ->
+      exists s', Lambda.multistep s1 s' /\ Lambda.multistep s2 s'.
+
+  Corollary Canonical_confluence : forall t t1 t2,
+      Canonical.multistep t t1 -> Canonical.multistep t t2 ->
+      exists t', Canonical.multistep t1 t' /\ Canonical.multistep t2 t'.
+  Proof.
+    intros t t1 t2 Htt1 Htt2.
+    apply θ_multistep_pres in Htt1.
+    apply θ_multistep_pres in Htt2.
+    specialize (Lambda_confluence _ _ _ Htt1 Htt2) as (s & H1s & H2s).
+    exists (ψ s). split.
+    - apply ψ_multistep_pres in H1s.
+      now rewrite (proj1 LambdaIsomorphism.inversion1) in H1s.
+    - apply ψ_multistep_pres in H2s.
+      now rewrite (proj1 LambdaIsomorphism.inversion1) in H2s.
+  Qed.
+
+  Corollary LambdaM_confluence : forall t t1 t2,
+    LambdaM.multistep t t1 -> LambdaM.multistep t t2 ->
+    exists t', LambdaM.multistep t1 t' /\ LambdaM.multistep t2 t'.
+  Proof.
+    intros t t1 t2 Htt1 Htt2.
+    apply conservativeness2' in Htt1.
+    apply conservativeness2' in Htt2.
+    specialize (Canonical_confluence _ _ _ Htt1 Htt2) as (t' & H1 & H2).
+    exists (i t'). split.
+    - apply conservativeness in H1.
+      rewrite (proj1 inversion1) in H1.
+      apply multistep_trans with (h t1).
+      + apply multistep_H_inclusion.
+        apply h_is_multistep_H.
+      + assumption.
+    - apply conservativeness in H2.
+      rewrite (proj1 inversion1) in H2.
+      apply multistep_trans with (h t2).
+      + apply multistep_H_inclusion.
+        apply h_is_multistep_H.
+      + assumption.
+  Qed.
+End Confluence.
